Add top level functions and the main and secondary theorems. There is no formal proof yet.

bft.v
@@ -5,17 +5,33 @@ Require Import Coq.Logic.FunctionalExtensionality.
 Require Import Coq.Lists.List.
 Import ListNotations.
 Require Import String.
+Require Import Maps.
 Open Scope string_scope.
 
-Definition total_map (A:Type) := string -> A.
-
-
-Definition Replica := string.
-Definition Ledger := string.
-
+Definition ReplicaId := string.
 Definition SysView := string.
-Definition SysState := string -> Ledger.
-Definition SysReplicas := string -> Replica.
+
+Inductive Message : Type := 
+| message: ReplicaId -> string -> Message.
+
+Notation "<< rId , pLoad >>" := (message rId pLoad).
+
+
+Definition get_rId (msg : Message) : ReplicaId :=
+  match msg with
+  | message x y => x
+  end.
+
+Definition get_pLoad (msg : Message) : string :=
+  match msg with
+  | message x y => y
+  end.
+
+Definition Ledger := total_map nat.
+Definition SysState := total_map Ledger.
+Definition MessageBox := list Message.
+Definition Replica := SysState -> Message -> MessageBox -> SysState.
+Definition SysReplicas := list (ReplicaId * Replica).
 
 Inductive System : Type := 
   | system : SysView -> SysState -> SysReplicas -> System.
@@ -35,11 +51,68 @@ Definition GetReplicas (sys : System) :=
   | system _ _ replicas => replicas
   end.
 
+Fixpoint findReplicaHelper (replicas : SysReplicas) (rId : ReplicaId) :=
+match replicas with
+| nil => None
+| (rId', r)::t => if beq_string rId rId' then (Some r)
+                  else findReplicaHelper t rId
+end.
 
-Definition State_empty : SysState :=  (fun _ => "None").
-Definition Replicas_empty : SysReplicas :=  (fun _ => "None").
+Definition FindReplica (sys : System) (rId:ReplicaId) :=
+let replicas := GetReplicas sys in
+  findReplicaHelper replicas rId.
 
-Check system.
 
-Definition system1 := (system "foo" State_empty Replicas_empty).
+Definition empty_ledger : Ledger :=  (fun _ => 0).
+Definition empty_state : SysState :=  (fun _ => empty_ledger).
+Definition empty_replicas : SysReplicas :=  nil.
+
+Definition ProcessMessage (sys:System) (rId : ReplicaId) (msg:Message) (msgBox : MessageBox) :=
+ match (FindReplica sys rId) with
+    | None => sys
+    | Some replica =>
+      let sysState' := (replica (GetState sys) msg msgBox) in
+        (system "foo" sysState' (GetReplicas sys))
+  end.
+
+Fixpoint ProcessAllMessages (sys:System) (msgBox: MessageBox) : System := 
+  match msgBox with
+  | nil => sys
+  | msg::t => let rId := get_rId msg in
+              let sys' := ProcessMessage sys rId msg msgBox in
+                ProcessAllMessages sys' t
+  end
+.
+
+Definition Request := string.
+
+Definition ProcessRequest (sys : System) (req : Request) :=
+  ProcessAllMessages sys [<<"foo", req>>].
+
+Definition NonFaulty (rId : ReplicaId) : Prop := True.
+Definition MajorityNonFaulty (sys:System) : Prop := True.
+
+Inductive StateValid : System -> Prop :=
+| empty_valid : forall sys:System, (GetState sys) = empty_state 
+                  -> StateValid sys.
+
+
+Lemma system_safety: forall (sys:System) (msgBox:MessageBox),
+  MajorityNonFaulty sys
+  -> StateValid (ProcessAllMessages sys msgBox)
+  -> forall (m:Message), StateValid (ProcessAllMessages sys (m::msgBox)).
+Proof. Admitted.
+
+
+Theorem byzantine_fault_tolerant : forall (sys:System) (msgBox : MessageBox),
+    MajorityNonFaulty sys 
+    -> StateValid sys
+    -> StateValid (ProcessAllMessages sys msgBox).
+Proof. intros. destruct sys as [view state replicas].
+induction msgBox. 
+  - simpl in H0. simpl. apply H0.
+  - induction replicas.
+    + apply IHmsgBox.
+    + apply system_safety; assumption.
+Qed.
 
