example-tests.v
@@ -1,0 +1,41 @@
+Require Import bft.
+Require Import Maps.
+Require Import Coq.Lists.List.
+Import ListNotations.
+
+Definition one_replicas : SysReplicas := ("foo", fun _ _ _ => empty_state)::empty_replicas.
+Definition system1 := (system "foo" empty_state one_replicas).
+Definition m1 := <<"foo", "1">>.
+Definition twoMsgBox := [m1 ; m1].
+
+Example sysEmptyTest : GetState (ProcessAllMessages system1 twoMsgBox) = empty_state.
+Proof. reflexivity. Qed.
+
+Example stValid_ProcMessages_sys1 : StateValid (ProcessAllMessages system1 twoMsgBox).
+Proof. constructor. reflexivity.   Qed.
+
+Print Replica.
+Print Ledger.
+
+Definition active_replicas : SysReplicas :=  
+      ("foo" , fun sysSt msg mb => sysSt & {"foo" --> (empty_ledger & { (get_pLoad msg) --> 1 }) } )
+      ::empty_replicas.
+Definition systemActive := (system "foo" empty_state active_replicas).
+Example stValid_ProcMessages_sysActive : StateValid (ProcessAllMessages systemActive twoMsgBox).
+Proof.  repeat apply system_safety; constructor; reflexivity.
+Qed.
+
+Definition multiple_active_replicas : SysReplicas :=
+      ("foo" , fun sysSt msg mb => sysSt & {"foo" --> (empty_ledger & { (get_pLoad msg) --> 1 }) } )
+      :: ("bar" , fun sysSt msg mb => sysSt & {"bar" --> (empty_ledger & { (get_pLoad msg) --> 1 }) } )
+      :: ("baz" , fun sysSt msg mb => sysSt & {"baz" --> (empty_ledger & { (get_pLoad msg) --> 1 }) } )
+      ::empty_replicas.
+
+Definition multi_replica_sys := (system "" empty_state multiple_active_replicas).
+Definition multi_replica_msgBox := [<<"foo", "1">> ; <<"bar" , "1">>; <<"baz" , "1">>].
+
+Example stValid_ProcMessages_multi_replicas : StateValid (ProcessAllMessages multi_replica_sys multi_replica_msgBox).
+Proof.  repeat apply system_safety; constructor; reflexivity.
+Qed.
+
+
